src/lib/kuiper/Kuiper.TensorCore.fst
@@ -1,0 +1,100 @@
+module Kuiper.TensorCore
+
+#lang-pulse
+
+open Kuiper
+open Pulse.Lib.Trade
+include Kuiper.TensorCore.Base
+
+ghost
+fn array_fragment_extract
+  (#et:Type0)
+  (#knd : fragment_kind)
+  (#m #n #k : nat)
+  (#l : fragment_layout)
+  (farr: array (fragment et knd m n k l))
+  // (#f : perm) // Assuming 1.0R for now
+  (ems : seq (value_for et knd m n k))
+  (i : natlt (Seq.length ems))
+  requires
+    array_fragment_pts_to farr ems
+  ensures
+    exists* (s : (lseq (fragment et knd m n k l) (Seq.length ems))).
+      farr |-> s **
+      (s @! i) |-> (ems @! i) **
+      (forall* (em' : value_for et knd m n k).
+        (farr |-> s **
+         (s @! i) |-> em') @==>
+          array_fragment_pts_to farr (Seq.upd ems i em'))
+{
+  unfold array_fragment_pts_to;
+  // Why "cannot find typeclass"?
+  // with s. assert farr |-> Frac f s;
+  with s. assert Pulse.Lib.Array.pts_to farr s;
+
+  forevery_extract_if_eqtype i
+    (fun (x : natlt (Seq.length s)) -> (s @! x) |-> (ems @! x));
+  
+  ghost
+  fn f_elim (em' : value_for et knd m n k)
+    requires
+      (forall+ (j : natlt (Seq.length ems)).
+        if op_Equality #(natlt (Seq.length ems)) j i then emp
+        else (s @! j) |-> (ems @! j))
+    ensures
+      (farr |-> s ** (s @! i) |-> em')
+      @==> array_fragment_pts_to farr (Seq.upd ems i em')
+  {
+    ghost
+    fn f_elim2 ()
+      requires
+        (forall+ (j : natlt (Seq.length ems)).
+          if op_Equality #(natlt (Seq.length ems)) j i then emp
+          else (s @! j) |-> (ems @! j)) **
+        (farr |-> s ** (s @! i) |-> em')
+      ensures
+        (array_fragment_pts_to farr (Seq.upd ems i em'))
+    {
+      let ems' = Seq.upd ems i em';
+      forevery_ext
+        (fun (j : natlt (Seq.length ems)) ->
+          if op_Equality #(natlt (Seq.length ems)) j i then emp
+          else (s @! j) |-> (ems @! j))
+        (fun (j : natlt (Seq.length ems')) ->
+          if op_Equality #(natlt (Seq.length ems)) j i then emp
+          else (s @! j) |-> (ems' @! j));
+      forevery_unextract_if_eqtype i _;
+      forevery_rw_type
+        (natlt (Seq.length ems))
+        (natlt (Seq.length ems'))
+        _;
+      fold array_fragment_pts_to farr ems';
+    };
+    intro_trade _ _ _ f_elim2;
+  };
+  intro_forall (forevery _ _) f_elim;
+  ();
+}
+
+ghost
+fn array_fragment_extract_ro
+  (#et:Type0)
+  (#knd : fragment_kind)
+  (#m #n #k : nat)
+  (#l : fragment_layout)
+  (farr: array (fragment et knd m n k l))
+  (ems : seq (value_for et knd m n k))
+  (#f : perm)
+  (i : natlt (Seq.length ems))
+  requires
+    array_fragment_pts_to farr #f ems
+  ensures
+    exists* (s : (lseq (fragment et knd m n k l) (Seq.length ems))).
+      factored
+        (farr |-> Frac f s ** (s @! i) |-> Frac f (ems @! i))
+        (array_fragment_pts_to farr #f ems)
+{
+  assume (pure (f == 1.0R));
+  array_fragment_extract farr ems i;
+  Pulse.Lib.Forall.elim_forall (ems @! i);
+}
